New evaluation rules

formal/SkLean/Eval.lean
@@ -5,8 +5,8 @@ namespace Expr
 def eval_once : Ast.Expr → Option Ast.Expr
   | SKM[((((K _α) _β) x) _y)] => pure x
   | SKM[((((((S _α) _β) _γ) x) y) z)] => pure SKM[((x z) (y z))]
-  | SKM[(((M K) α) β)]     => pure SKM[(α ~> (β ~> α))]
-  | SKM[((((M S) α) β) γ)] => pure SKM[(α ~> β ~> γ ~> ((α γ) (β γ)))]
+  | SKM[(((M K) α) β)]     => pure SKM[(α ~> (β ~> (((K (M β)) α) β)))]
+  | SKM[((((M S) α) β) γ)] => pure SKM[(α ~> β ~> γ ~> (((((S (M α)) (M β)) γ) α) β))]
   | SKM[((M M) K)] => pure SKM[Prp]
   | SKM[((M M) S)] => pure SKM[Prp]
   | SKM[((M M) M)] => pure SKM[Prp]
@@ -26,5 +26,11 @@ def eval_n : ℕ → Ast.Expr → Option Ast.Expr
     eval_n n e'
 
 end Expr
+
+inductive IsEvalOnce : Ast.Expr → Ast.Expr → Prop
+  | k   : IsEvalOnce SKM[((((K _α) _β) x) y)] x
+  | s   : IsEvalOnce SKM[((((((S _α) _β) _γ) x) y) z)] SKM[((x z) (y z))]
+  | m_k : IsEvalOnce SKM[(((M K) α) β)] SKM[(α ~> β ~> α)]
+  | m_s : IsEvalOnce SKM[((((M S) α) β) γ)] SKM[(α ~> β ~> γ ~> ((α γ) (β γ)))]
 
 def BetaEq := Relation.ReflTransGen (λ x y => Expr.eval_once x = .some y ∨ Expr.eval_once y = .some x)
